books/kestrel/utilities/fixbytes/defbytelist-tests.lisp
@@ -20,21 +20,21 @@
 
 (must-succeed*
  (fty::defbyte ubyte8 :size 8)
- (fty::defbytelist ubyte8-list ubyte8)
+ (fty::defbytelist ubyte8-list :elt-type ubyte8)
  (assert! (function-symbolp 'ubyte8-list-p (w state)))
  (assert! (function-symbolp 'ubyte8-list-fix$inline (w state)))
  (assert! (function-symbolp 'ubyte8-list-equiv$inline (w state))))
 
 (must-succeed*
  (fty::defbyte word :size 16)
- (fty::defbytelist word-list word)
+ (fty::defbytelist word-list :elt-type word)
  (assert! (function-symbolp 'word-list-p (w state)))
  (assert! (function-symbolp 'word-list-fix$inline (w state)))
  (assert! (function-symbolp 'word-list-equiv$inline (w state))))
 
 (must-succeed*
  (fty::defbyte sbyte1 :size 1 :signed t)
- (fty::defbytelist sbyte1-list sbyte1)
+ (fty::defbytelist sbyte1-list :elt-type sbyte1)
  (assert! (function-symbolp 'sbyte1-list-p (w state)))
  (assert! (function-symbolp 'sbyte1-list-fix$inline (w state)))
  (assert! (function-symbolp 'sbyte1-list-equiv$inline (w state))))
@@ -42,7 +42,7 @@
 (must-succeed*
  (defconst *size* 100)
  (fty::defbyte ubyte100 :size *size*)
- (fty::defbytelist ubyte100-list ubyte100)
+ (fty::defbytelist ubyte100-list :elt-type ubyte100)
  (assert! (function-symbolp 'ubyte100-list-p (w state)))
  (assert! (function-symbolp 'ubyte100-list-fix$inline (w state)))
  (assert! (function-symbolp 'ubyte100-list-equiv$inline (w state))))
@@ -50,7 +50,7 @@
 (must-succeed*
  (define size () 50)
  (fty::defbyte mybyte :size (size))
- (fty::defbytelist mybyte-list mybyte)
+ (fty::defbytelist mybyte-list :elt-type mybyte)
  (assert! (function-symbolp 'mybyte-list-p (w state)))
  (assert! (function-symbolp 'mybyte-list-fix$inline (w state)))
  (assert! (function-symbolp 'mybyte-list-equiv$inline (w state))))
@@ -61,7 +61,7 @@
    (local (defun size () 2))
    (defthm posp-of-size (posp (size))))
  (fty::defbyte mybyte :size (size))
- (fty::defbytelist mybyte-list mybyte)
+ (fty::defbytelist mybyte-list :elt-type mybyte)
  (assert! (function-symbolp 'mybyte-list-p (w state)))
  (assert! (function-symbolp 'mybyte-list-fix$inline (w state)))
  (assert! (function-symbolp 'mybyte-list-equiv$inline (w state))))
@@ -72,11 +72,11 @@
 
 (must-succeed*
  (fty::defbyte ubyte4 :size 4)
- (must-fail (fty::defbytelist #\A ubyte4)))
+ (must-fail (fty::defbytelist #\A :elt-type ubyte4)))
 
 (must-succeed*
  (fty::defbyte ubyte4 :size 4)
- (fty::defbytelist nibbles ubyte4)
+ (fty::defbytelist nibbles :elt-type ubyte4)
  (assert! (function-symbolp 'nibbles-p (w state)))
  (assert! (function-symbolp 'nibbles-fix$inline (w state)))
  (assert! (function-symbolp 'nibbles-equiv$inline (w state))))
@@ -85,21 +85,21 @@
 
 ; test the BYTE input:
 
-(must-fail (fty::defbytelist byte-list "string"))
+(must-fail (fty::defbytelist byte-list :elt-type "string"))
 
-(must-fail (fty::defbytelist byte-list (#\x 3/4)))
+(must-fail (fty::defbytelist byte-list :elt-type (#\x 3/4)))
 
-(must-fail (fty::defbytelist byte-list not-even-a-fixtype))
+(must-fail (fty::defbytelist byte-list :elt-type not-even-a-fixtype))
 
-(must-fail (fty::defbytelist byte-list nat))
+(must-fail (fty::defbytelist byte-list :elt-type nat))
 
 (must-succeed*
  (fty::defbyte mybyte :size 8)
- (must-fail (fty::defbytelist mybyte-list mybyt)))
+ (must-fail (fty::defbytelist mybyte-list :elt-type mybyt)))
 
 (must-succeed*
  (fty::defbyte mybyte :size 5)
- (fty::defbytelist mybyte-list mybyte)
+ (fty::defbytelist mybyte-list :elt-type mybyte)
  (assert! (mybyte-list-p '(0 1 31)))
  (assert! (not (mybyte-list-p '(32)))))
 
@@ -109,11 +109,11 @@
 
 (must-succeed*
  (fty::defbyte byte :size 4)
- (must-fail (fty::defbytelist bytes byte :pred 888)))
+ (must-fail (fty::defbytelist bytes :elt-type byte :pred 888)))
 
 (must-succeed*
  (fty::defbyte ubyte4 :size 4)
- (fty::defbytelist ubyte4-list ubyte4 :pred nibblesp)
+ (fty::defbytelist ubyte4-list :elt-type ubyte4 :pred nibblesp)
  (assert! (function-symbolp 'nibblesp (w state)))
  (assert! (function-symbolp 'ubyte4-list-fix$inline (w state)))
  (assert! (function-symbolp 'ubyte4-list-equiv$inline (w state))))
@@ -124,11 +124,11 @@
 
 (must-succeed*
  (fty::defbyte byte :size 4)
- (must-fail (fty::defbytelist bytes byte :fix #c(1 2))))
+ (must-fail (fty::defbytelist bytes :elt-type byte :fix #c(1 2))))
 
 (must-succeed*
  (fty::defbyte ubyte4 :size 4)
- (fty::defbytelist ubyte4-list ubyte4 :fix nibfix)
+ (fty::defbytelist ubyte4-list :elt-type ubyte4 :fix nibfix)
  (assert! (function-symbolp 'ubyte4-list-p (w state)))
  (assert! (function-symbolp 'nibfix$inline (w state)))
  (assert! (function-symbolp 'ubyte4-list-equiv$inline (w state))))
@@ -139,11 +139,11 @@
 
 (must-succeed*
  (fty::defbyte ubyte4 :size 4)
- (must-fail (fty::defbytelist ubyte4-list ubyte4 :equiv (1 1 1))))
+ (must-fail (fty::defbytelist ubyte4-list :elt-type ubyte4 :equiv (1 1 1))))
 
 (must-succeed*
  (fty::defbyte ubyte4 :size 4)
- (fty::defbytelist ubyte4-list ubyte4 :equiv nibeq)
+ (fty::defbytelist ubyte4-list :elt-type ubyte4 :equiv nibeq)
  (assert! (function-symbolp 'ubyte4-list-p (w state)))
  (assert! (function-symbolp 'ubyte4-list-fix$inline (w state)))
  (assert! (function-symbolp 'nibeq$inline (w state))))
@@ -154,15 +154,15 @@
 
 (must-succeed*
  (fty::defbyte byte :size 4)
- (must-fail (fty::defbytelist byte-list byte :parents one)))
+ (must-fail (fty::defbytelist byte-list :elt-type byte :parents one)))
 
 (must-succeed*
  (fty::defbyte byte :size 4)
- (fty::defbytelist byte-list byte :parents nil))
+ (fty::defbytelist byte-list :elt-type byte :parents nil))
 
 (must-succeed*
  (fty::defbyte byte :size 4)
- (fty::defbytelist byte-list byte :parents (this that)))
+ (fty::defbytelist byte-list :elt-type byte :parents (this that)))
 
 ;;;;;;;;;;;;;;;;;;;;;;;;;;;;;;;;;;;;;;;;;;;;;;;;;;;;;;;;;;;;;;;;;;;;;;;;;;;;;;;;
 
@@ -170,15 +170,17 @@
 
 (must-succeed*
  (fty::defbyte byte :size 4)
- (must-fail (fty::defbytelist bytes byte :short #\s)))
+ (must-fail (fty::defbytelist bytes :elt-type byte :short #\s)))
 
 (must-succeed*
  (fty::defbyte byte :size 4)
- (fty::defbytelist bytes byte :short "Short doc."))
+ (fty::defbytelist bytes :elt-type byte :short "Short doc."))
 
 (must-succeed*
  (fty::defbyte byte :size 4)
- (fty::defbytelist bytes byte :short (concatenate 'string "Short" " " "doc.")))
+ (fty::defbytelist bytes
+                   :elt-type byte
+                   :short (concatenate 'string "Short" " " "doc.")))
 
 ;;;;;;;;;;;;;;;;;;;;;;;;;;;;;;;;;;;;;;;;;;;;;;;;;;;;;;;;;;;;;;;;;;;;;;;;;;;;;;;;
 
@@ -186,12 +188,14 @@
 
 (must-succeed*
  (fty::defbyte byte :size 4)
- (must-fail (fty::defbytelist bytes byte :long (#\t #\o #\p #\i #\c))))
+ (must-fail (fty::defbytelist bytes
+                              :elt-type byte
+                              :long (#\t #\o #\p #\i #\c))))
 
 (must-succeed*
  (fty::defbyte byte :size 4)
- (fty::defbytelist bytes byte :long "<p>More doc.</p>"))
+ (fty::defbytelist bytes :elt-type byte :long "<p>More doc.</p>"))
 
 (must-succeed*
  (fty::defbyte byte :size 4)
- (fty::defbytelist bytes byte :long (xdoc::toppstring "More doc.")))
+ (fty::defbytelist bytes :elt-type byte :long (xdoc::toppstring "More doc.")))
